# Exercise 5: Multiplying Complex Numbers

Practice problems for Lesson 5. Use FOIL and remember $i^2 = -1$!

---

## Part A: Basic Multiplication

**Multiply using FOIL:**

1. $(2 + i)(3 + i)$
2. $(4 + 2i)(1 + 3i)$
3. $(5 + i)(2 + i)$
4. $(3 + 4i)(2 + i)$
5. $(1 + i)(1 + 2i)$

---

## Part B: Multiplication with Negatives

**Watch the signs carefully:**

6. $(3 - i)(2 + i)$
7. $(4 + 2i)(3 - i)$
8. $(5 - 2i)(1 - 3i)$
9. $(-2 + i)(3 + 2i)$
10. $(-1 - i)(2 - 3i)$

---

## Part C: Multiplying by Real Numbers

**Distribute the real number:**

11. $3(2 + 5i)$
12. $-4(1 - 3i)$
13. $5(3 + 2i)$
14. $-2(-4 + 7i)$

---

## Part D: Multiplying by Pure Imaginary Numbers

**Simplify completely:**

15. $2i(3 + 4i)$
16. $5i(2 - i)$
17. $-3i(1 + 2i)$
18. $i(4 - 5i)$

---

## Part E: Multiplying by $i$

**Quick transformation:**

19. $(3 + 4i) \times i$
20. $(5 - 2i) \times i$
21. $(7 + i) \times i$
22. $(-2 + 6i) \times i$

---

## Part F: Multiplying by Conjugates

**These should give real answers:**

23. $(3 + 4i)(3 - 4i)$
24. $(2 + 5i)(2 - 5i)$
25. $(1 + i)(1 - i)$
26. $(5 - 3i)(5 + 3i)$
27. $(7 + i)(7 - i)$

---

## Part G: Squaring Complex Numbers

**Calculate $(z)^2$:**

28. $(1 + i)^2$
29. $(2 + 3i)^2$
30. $(3 - i)^2$
31. $(4 - 2i)^2$
32. $(1 - 2i)^2$

---

## Part H: Three Factor Products

**Multiply step by step:**

33. $(1 + i)(1 + i)(1 - i)$
34. $(2 + i)(1 - i)(2 - i)$
35. $i(2 + 3i)(1 - i)$

---

## Part I: Using the Formula

**Use $(a + bi)^2 = (a^2 - b^2) + 2abi$:**

36. $(5 + 2i)^2$
37. $(3 + 4i)^2$
38. $(6 - i)^2$

---

## Part J: Absolute Value Properties

**Calculate $|z_1 \times z_2|$ two ways:**

39. $|(2 + i)(1 + 2i)|$ 
    Method 1: Multiply first, then find modulus
    Method 2: $|z_1| \times |z_2|$

40. $|(3 + 4i)(1 - i)|$
    Use both methods

---

## Part K: Mixed Operations

41. $(2 + i)(3 - i) + (1 + 2i)$
42. $(4 - 3i)(1 + i) - (2 - i)$
43. $2(3 + i) + (1 - i)(2 + i)$

---

## Part L: Challenge Problems

44. $(1 + i)^4$ [Hint: $(1 + i)^2$ first, then square that]
45. $(2 - i)^3$ [Hint: $(2 - i)^2$ first, then multiply by $(2 - i)$]
46. $\frac{(3 + 4i)(2 - i)}{5}$ [Multiply numerator first, then divide]
47. $(a + bi)(a + bi)$ where $a = 1$ and $b = 1$
48. Show that $(z)(z) = |z|^2$ for $z = 3 + 4i$

---

## Solutions

### Part A Solutions
1. $(2 + i)(3 + i) = 6 + 2i + 3i + i^2 = 6 + 5i - 1 = 5 + 5i$
2. $(4 + 2i)(1 + 3i) = 4 + 12i + 2i + 6i^2 = 4 + 14i - 6 = -2 + 14i$
3. $(5 + i)(2 + i) = 10 + 5i + 2i + i^2 = 10 + 7i - 1 = 9 + 7i$
4. $(3 + 4i)(2 + i) = 6 + 3i + 8i + 4i^2 = 6 + 11i - 4 = 2 + 11i$
5. $(1 + i)(1 + 2i) = 1 + 2i + i + 2i^2 = 1 + 3i - 2 = -1 + 3i$

### Part B Solutions
6. $(3 - i)(2 + i) = 6 + 3i - 2i - i^2 = 6 + i + 1 = 7 + i$
7. $(4 + 2i)(3 - i) = 12 - 4i + 6i - 2i^2 = 12 + 2i + 2 = 14 + 2i$
8. $(5 - 2i)(1 - 3i) = 5 - 15i - 2i + 6i^2 = 5 - 17i - 6 = -1 - 17i$
9. $(-2 + i)(3 + 2i) = -6 - 4i + 3i + 2i^2 = -6 - i - 2 = -8 - i$
10. $(-1 - i)(2 - 3i) = -2 + 3i - 2i + 3i^2 = -2 + i - 3 = -5 + i$

### Part C Solutions
11. $3(2 + 5i) = 6 + 15i$
12. $-4(1 - 3i) = -4 + 12i$
13. $5(3 + 2i) = 15 + 10i$
14. $-2(-4 + 7i) = 8 - 14i$

### Part D Solutions
15. $2i(3 + 4i) = 6i + 8i^2 = 6i - 8 = -8 + 6i$
16. $5i(2 - i) = 10i - 5i^2 = 10i + 5 = 5 + 10i$
17. $-3i(1 + 2i) = -3i - 6i^2 = -3i + 6 = 6 - 3i$
18. $i(4 - 5i) = 4i - 5i^2 = 4i + 5 = 5 + 4i$

### Part E Solutions
19. $(3 + 4i) \times i = 3i + 4i^2 = 3i - 4 = -4 + 3i$
20. $(5 - 2i) \times i = 5i - 2i^2 = 5i + 2 = 2 + 5i$
21. $(7 + i) \times i = 7i + i^2 = 7i - 1 = -1 + 7i$
22. $(-2 + 6i) \times i = -2i + 6i^2 = -2i - 6 = -6 - 2i$

### Part F Solutions (All Real!)
23. $(3 + 4i)(3 - 4i) = 9 + 16 = 25$
24. $(2 + 5i)(2 - 5i) = 4 + 25 = 29$
25. $(1 + i)(1 - i) = 1 + 1 = 2$
26. $(5 - 3i)(5 + 3i) = 25 + 9 = 34$
27. $(7 + i)(7 - i) = 49 + 1 = 50$

### Part G Solutions
28. $(1 + i)^2 = 1 + 2i + i^2 = 1 + 2i - 1 = 2i$
29. $(2 + 3i)^2 = 4 + 12i + 9i^2 = 4 + 12i - 9 = -5 + 12i$
30. $(3 - i)^2 = 9 - 6i + i^2 = 9 - 6i - 1 = 8 - 6i$
31. $(4 - 2i)^2 = 16 - 16i + 4i^2 = 16 - 16i - 4 = 12 - 16i$
32. $(1 - 2i)^2 = 1 - 4i + 4i^2 = 1 - 4i - 4 = -3 - 4i$

### Part H Solutions
33. $(1 + i)^2(1 - i) = 2i(1 - i) = 2i - 2i^2 = 2i + 2 = 2 + 2i$
34. $(2 + i)(1 - i)(2 - i) = (2 - 2i + i - i^2)(2 - i) = (3 - i)(2 - i) = 6 - 3i - 2i + i^2 = 5 - 5i$
35. $i(2 + 3i)(1 - i) = i(2 - 2i + 3i - 3i^2) = i(5 + i) = 5i + i^2 = -1 + 5i$

### Part I Solutions
36. $(5 + 2i)^2 = (25 - 4) + 20i = 21 + 20i$
37. $(3 + 4i)^2 = (9 - 16) + 24i = -7 + 24i$
38. $(6 - i)^2 = (36 - 1) - 12i = 35 - 12i$

### Part J Solutions
39. **Method 1:** $(2 + i)(1 + 2i) = 2 + 4i + i + 2i^2 = 5i$, so $|5i| = 5$
    **Method 2:** $|2 + i| = \sqrt{5}$, $|1 + 2i| = \sqrt{5}$, so $\sqrt{5} \times \sqrt{5} = 5$ ✓

40. **Method 1:** $(3 + 4i)(1 - i) = 3 - 3i + 4i - 4i^2 = 7 + i$, so $|7 + i| = \sqrt{50} = 5\sqrt{2}$
    **Method 2:** $|3 + 4i| = 5$, $|1 - i| = \sqrt{2}$, so $5 \times \sqrt{2} = 5\sqrt{2}$ ✓

### Part K Solutions
41. $(2 + i)(3 - i) + (1 + 2i) = (6 - 2i + 3i - i^2) + (1 + 2i) = (7 + i) + (1 + 2i) = 8 + 3i$
42. $(4 - 3i)(1 + i) - (2 - i) = (4 + 4i - 3i - 3i^2) - (2 - i) = (7 + i) - (2 - i) = 5 + 2i$
43. $2(3 + i) + (1 - i)(2 + i) = (6 + 2i) + (2 + i - 2i - i^2) = (6 + 2i) + (3 - i) = 9 + i$

### Part L Solutions
44. $(1 + i)^2 = 2i$, then $(2i)^2 = 4i^2 = -4$

45. $(2 - i)^2 = 4 - 4i + i^2 = 3 - 4i$
    $(3 - 4i)(2 - i) = 6 - 3i - 8i + 4i^2 = 2 - 11i$

46. $(3 + 4i)(2 - i) = 6 - 3i + 8i - 4i^2 = 10 + 5i$
    $\frac{10 + 5i}{5} = 2 + i$

47. $(1 + i)(1 + i) = 1 + 2i + i^2 = 2i$

48. $(3 + 4i)(3 - 4i) = 9 + 16 = 25$
    $|3 + 4i|^2 = (\sqrt{25})^2 = 25$ ✓ (They're equal!)

---

## How Did You Do?

- **45-48 correct:** Spectacular! You're a multiplication master!
- **38-44 correct:** Excellent! Ready for division.
- **30-37 correct:** Good work! Practice FOIL more.
- **Below 30:** Review Lesson 5, especially $i^2 = -1$.

**Next:** Open `Lesson_6_Dividing_Complex_Numbers.md` for the final lesson!
